worked on execution utils

coq/Fragment.v
@@ -215,5 +215,446 @@ apply (pc_in_range _ _ code loc1 loc2 (PUSH1 loc1::JUMPI::PUSH1 loc2 :: JUMP :: 
 apply N.leb_le;auto.
 
 Qed.
+
+Definition in_locN v c loc :=
+  N.eqb (loc + program_length v.(venv_prg_sfx))
+          (program_length c.(cenv_program)).
+
+Lemma bool_tf : forall b, b=false \/ b = true.
+destruct b;auto.
+Qed.
+
+Lemma break_condition : forall steps v1 v2 c cond,
+   FragmentContinue v2 = fragment_sem cond v1 c steps ->
+   cond v2 = true.
+induction steps.
+simpl.
+intros.
+inversion H.
+simpl.
+intros.
+
+elim (bool_tf (cond v1));intros;rewrite H0 in H.
+
+destruct (venv_prg_sfx v1).
+
+inversion H.
+destruct (instruction_sem v1 c i); try inversion H.
+eapply IHsteps.
+eassumption.
+destruct c0; try inversion H.
+
+destruct o; inversion H.
+inversion H; trivial.
+Qed.
+
+Lemma runout_dec : forall res,
+  FragmentStepRunOut = res \/ FragmentStepRunOut <> res.
+intros.
+destruct res; try (right ; congruence).
+left; auto.
+Qed.
+
+Lemma can_continue :
+  forall steps v c cond vv,
+  FragmentContinue vv = fragment_sem cond v c (S steps) ->
+  FragmentStepRunOut <> fragment_sem cond v c steps ->
+  FragmentContinue vv = fragment_sem cond v c steps.
+induction steps; intros.
+simpl in H0.
+congruence.
+assert (H' := H).
+simpl; simpl in H, H0.
+elim (bool_tf (cond v)); intros.
+rewrite H1 in *.
+destruct (venv_prg_sfx v).
+inversion H.
+destruct (instruction_sem v c i).
+apply IHsteps;auto.
+destruct c0; try congruence.
+congruence.
+rewrite H1 in *.
+trivial.
+Qed.
+
+Lemma smallest_steps : forall steps v c cond vv,
+   FragmentContinue vv = fragment_sem cond v c steps ->
+   exists ss,
+   FragmentContinue vv = fragment_sem cond v c (S ss) /\
+   FragmentStepRunOut = fragment_sem cond v c ss.
+intros.
+induction steps.
+inversion H.
+elim (runout_dec (fragment_sem cond v c steps)); intros.
+exists steps; auto.
+apply IHsteps.
+
+destruct steps.
+simpl in H0.
+congruence.
+simpl in *.
+elim (bool_tf (cond v)); intros.
+rewrite H1 in *.
+destruct (venv_prg_sfx v).
+inversion H.
+destruct (instruction_sem v c i).
+
+apply can_continue; auto.
+congruence.
+congruence.
+rewrite H1 in *.
+trivial.
+Qed.
+
+Lemma add_useless_step : forall steps v c cond vv,
+  FragmentContinue vv = fragment_sem cond v c steps -> 
+  FragmentContinue vv = fragment_sem cond v c (S steps).
+induction steps; intros.
+simpl in H; inversion H.
+unfold fragment_sem; fold fragment_sem.
+unfold fragment_sem in H; fold fragment_sem in H.
+elim (bool_tf (cond v)); intros; rewrite H0 in *; auto.
+destruct (venv_prg_sfx v).
+inversion H.
+
+destruct (instruction_sem v c i); try inversion H.
+apply IHsteps; auto.
+destruct c0; try inversion H.
+destruct o; inversion H.
+Qed.
+
+Lemma add_useless_steps : forall n steps v c cond vv1 vv2,
+  FragmentContinue vv1 = fragment_sem cond v c (steps+n) -> 
+  FragmentContinue vv2 = fragment_sem cond v c steps ->
+  vv1 = vv2.
+induction n; intros.
+Search (_ + 0 = _)%nat.
+rewrite Nat.add_0_r in H.
+congruence.
+apply (IHn (S steps) v c cond); auto.
+replace (S steps + n)%nat with (steps + S n)%nat; auto.
+omega.
+apply add_useless_step.
+auto.
+Qed.
+
+Lemma add_steps_same : forall steps1 steps2 v c cond vv1 vv2,
+  FragmentContinue vv1 = fragment_sem cond v c steps1 -> 
+  FragmentContinue vv2 = fragment_sem cond v c steps2 ->
+  vv1 = vv2.
+intros.
+elim (Nat.add_dichotomy steps1 steps2); intros.
+elim H1; clear H1; intros.
+rewrite <- H1 in H0.
+apply eq_sym.
+eapply add_useless_steps; try rewrite Nat.add_comm; eassumption.
+elim H1; clear H1; intros.
+rewrite <- H1 in H.
+eapply add_useless_steps; try rewrite Nat.add_comm; eassumption.
+Qed.
+
+Lemma break_weaker : forall (P:variable_env -> Prop) cond1 cond2,
+   (forall v, cond1 v = true -> cond2 v = true) ->
+    forall steps v c vv,
+    cond1 vv = true ->
+    FragmentContinue vv = fragment_sem cond2 v c steps ->
+    FragmentContinue vv = fragment_sem cond1 v c steps.
+
+induction steps; intros.
+simpl in H1; inversion H1.
+
+simpl.
+simpl in H1.
+
+elim (bool_tf (cond1 v)); elim (bool_tf (cond2 v)); intros;
+ rewrite H2 in *; rewrite H3 in *.
+
+destruct (venv_prg_sfx v).
+inversion H1.
+
+destruct (instruction_sem v c i); try inversion H.
+
+apply IHsteps; auto.
+
+destruct c; destruct o; inversion H1;auto.
+
+inversion H1.
+
+inversion H1.
+rewrite H5 in *.
+rewrite H3 in H0.
+congruence.
+
+rewrite H in H2; congruence.
+assumption.
+Qed.
+
+Fixpoint iter_sem v c steps :=
+  match steps with
+    | O => FragmentContinue v
+    | S remaining_steps =>
+      match v.(venv_prg_sfx) with
+      | nil => FragmentToWorld ContractFail v.(venv_storage_at_call) v.(venv_balance_at_call) None
+      | i :: _ =>
+        match instruction_sem v c i with
+        | InstructionContinue new_v =>
+          iter_sem new_v c remaining_steps
+        | InstructionToWorld ContractFail opt_pushed_v =>
+          FragmentToWorld ContractFail v.(venv_storage_at_call) v.(venv_balance_at_call) opt_pushed_v
+        | InstructionToWorld (ContractCall args) (Some new_v) =>
+          FragmentToWorld (ContractCall args) new_v.(venv_storage) new_v.(venv_balance) (Some new_v)
+        | InstructionToWorld a opt_pushed_v =>
+          FragmentToWorld a v.(venv_storage) v.(venv_balance) opt_pushed_v
+        | InstructionInvalid => FragmentInvalid
+        end
+      end
+  end.
+
+Lemma run_out_less : forall steps v c cond,
+  FragmentStepRunOut = fragment_sem cond v c (S steps) ->
+  FragmentStepRunOut = fragment_sem cond v c steps.
+induction steps; intros; auto.
+simpl.
+simpl in H.
+elim (bool_tf (cond v)); intros.
+rewrite H0 in *.
+destruct (venv_prg_sfx v); auto.
+destruct (instruction_sem v c i).
+apply IHsteps.
+auto.
+destruct c0; destruct o; inversion H.
+inversion H.
+rewrite H0 in *.
+inversion H.
+Qed.
+
+Lemma iter_cond : forall steps v c cond vv,
+   FragmentStepRunOut = fragment_sem cond v c (S steps) ->
+   FragmentContinue vv = iter_sem v c steps ->
+   cond vv = false.
+induction steps; intros.
+simpl in *.
+inversion H0.
+rewrite H2 in *.
+elim (bool_tf (cond v)); intros; auto.
+rewrite H1 in *.
+inversion H.
+
+simpl in H, H0.
+
+elim (bool_tf (cond v)); intros; auto.
+rewrite H1 in *.
+
+destruct (venv_prg_sfx v).
+inversion H.
+destruct (instruction_sem v c i).
+apply (IHsteps v0 c);auto.
+
+destruct c0; destruct o; inversion H.
+inversion H.
+rewrite H1 in *.
+inversion H.
+Qed.
+
+Lemma iter_seq : forall steps v c vv,
+   FragmentContinue vv = iter_sem v c (S steps) ->
+   exists v2, FragmentContinue v2 = iter_sem v c steps.
+induction steps; intros.
+simpl.
+exists v; auto.
+simpl; simpl in H.
+destruct (venv_prg_sfx v).
+inversion H.
+destruct (instruction_sem v c i).
+elim (IHsteps v0 c vv).
+intros.
+exists x; auto.
+auto.
+destruct c0; destruct o; inversion H.
+inversion H.
+Qed.
+
+Lemma iter_seq_add : forall n steps v c vv,
+   FragmentContinue vv = iter_sem v c (n + steps) ->
+   exists v2, FragmentContinue v2 = iter_sem v c steps.
+induction n; intros.
+simpl in H.
+exists vv; auto.
+eelim (iter_seq (n+steps) v c); intros.
+eapply IHn.
+exact H0.
+replace (S (n + steps))%nat with (S n + steps)%nat.
+eassumption.
+omega.
+Qed.
+
+Lemma iter_seq_all : forall n steps v c vv,
+   (n < steps)%nat ->
+   FragmentContinue vv = iter_sem v c steps ->
+   exists v2, FragmentContinue v2 = iter_sem v c n.
+intros.
+elim (Nat.add_dichotomy steps n); intros.
+elim H1; intros; omega.
+elim H1; clear H1; intros.
+eapply iter_seq_add.
+rewrite H1.
+eassumption.
+Qed.
+
+
+Lemma iter_cond_true : forall steps v c cond vv,
+   FragmentContinue vv = iter_sem v c steps ->
+   cond vv = true ->
+   (forall v2 n, (n < steps)%nat -> FragmentContinue v2 = iter_sem v c n ->
+    cond vv = false) ->
+   FragmentContinue vv = fragment_sem cond v c (S steps).
+induction steps; intros.
+simpl.
+simpl in H.
+inversion H.
+rewrite H2 in *.
+rewrite H0.
+trivial.
+
+elim (bool_tf (cond v)); intros; auto.
+simpl; simpl in H.
+rewrite H1 in *.
+
+destruct (venv_prg_sfx v).
+inversion H.
+destruct (instruction_sem v c i).
+apply (IHsteps v0 c);auto.
+
+destruct c0; destruct o; inversion H.
+inversion H.
+
+
+simpl; simpl in H.
+rewrite H1 in *.
+
+destruct (venv_prg_sfx v).
+inversion H.
+destruct (instruction_sem v c i).
+pose (IHsteps v0 c cond vv H H0);auto.
+simpl in e.
+elim (bool_tf (cond v0)); intros; auto.
+rewrite H2 in *.
+
+destruct (venv_prg_sfx v0).
+inversion e.
+destruct (instruction_sem v0 c i0).
+apply (IHsteps v1 c);auto.
+
+destruct c0; destruct o; inversion H.
+inversion H.
+
+
+rewrite H1 in *.
+inversion H.
+Qed.
+
+
+Lemma iter_fragment : forall steps v c cond vv,
+   FragmentContinue vv = fragment_sem cond v c steps ->
+   exists n, iter_sem v c n = fragment_sem cond v c steps.
+intros.
+elim (smallest_steps steps v c cond vv H); intros.
+elim H0; clear H0; intros.
+exists (S x).
+induction x.
+simpl in *.
+
+
+
+Lemma iter_smallest_fragment : forall n v c cond vv,
+   FragmentContinue vv = fragment_sem cond v c (S n) ->
+   FragmentStepRunOut = fragment_sem cond v c n ->
+   cond v = false ->
+   iter_sem v c (S n) = fragment_sem cond v c (S n).
+
+
+
+Lemma iter_smallest_fragment_O : forall v c cond vv,
+   FragmentContinue vv = fragment_sem cond v c (S O) ->
+   cond v = false ->
+   iter_sem v c (S O) = fragment_sem cond v c (S O).
+intros.
+simpl in H.
+simpl.
+rewrite !H0 in *.
+destruct (venv_prg_sfx v); auto.
+destruct (instruction_sem v c i).
+inversion H.
+destruct c0; destruct o; inversion H.
+inversion H.
+Qed.
+
+
+induction n; intros.
+eapply iter_smallest_fragment_O; eassumption.
+
+rewrite <- H.
+simpl.
+simpl in H.
+rewrite !H1 in *.
+destruct (venv_prg_sfx v); auto.
+destruct (instruction_sem v c i).
+
+simpl in H; simpl.
+
+simpl in H0.
+rewrite !H1 in *.
+rewrite H1.
+
+Lemma iter_fragment_step : forall steps v c cond vv,
+    FragmentContinue vv = fragment_sem cond v c (S steps) ->
+    FragmentStepRunOut = fragment_sem cond v c steps ->
+   cond v = false ->
+   iter_sem v c (S steps) = fragment_sem cond v c (S steps).
+
+
+
+induction steps; intros.
+simpl in H; inversion H.
+simpl in H.
+elim (bool_tf (cond v)); intros.
+rewrite H0 in *.
+destruct (venv_prg_sfx v).
+inversion H.
+destruct (instruction_sem v c i).
+apply (IHsteps v c cond).
+
+(* Needs to specify that it stays in fragment *)
+Lemma compose_simple_fragments :
+  forall (Pre P2 Post: variable_env -> Prop) c steps1 steps2 v code1 code2 rest,
+  v.(venv_prg_sfx) = code1 ++ code2 ++ rest -> 
+  (forall v1 rest1 c1,
+     v1.(venv_prg_sfx) = code1 ++ rest1 -> 
+     Pre v1 ->
+     exists vv, P2 vv /\
+     in_locN v c1 (pc v1 + program_length code1) = true /\
+     FragmentContinue vv = fragment_sem (fun v =>
+       in_locN v c1 (pc v1 + program_length code1) ||
+       in_locN v c1 (pc v1 + program_length code1 + program_length code2))%bool v1 c steps1) ->
+  (forall v2 rest2 c2,
+     v2.(venv_prg_sfx) = code2 ++ rest2 -> 
+     P2 v2 ->
+     exists vv, Post vv /\
+     FragmentContinue vv =
+     fragment_sem (fun v => in_locN v c2 (pc v2 + program_length code2)) v2 c steps2) ->
+  Pre v -> exists vv, Post vv /\
+  FragmentContinue vv =
+  fragment_sem (fun v' => in_locN v' c (pc v + program_length code1 + program_length code2)) v c (steps1 + steps2).
+intros.
+elim (H0 v (code2++rest) c H H2); intros.
+clear H0.
+elim H3; clear H3; intros.
+elim H3; clear H3; intros.
+elim (H1 x rest c); intros; auto.
+elim H5; clear H5; intros.
+exists x0.
+split; auto.
+clear H1.
+
 End Fragment.
 
